cava/Cava/Lib/RetimingProperties.v
@@ -28,909 +28,319 @@ Require Import Cava.Semantics.WeakEquivalence.
 Require Import Cava.Lib.CircuitTransforms.
 Require Import Cava.Lib.CircuitTransformsProperties.
 Require Import Cava.Lib.Retiming.
+Require Import Cava.Lib.Multiplexers.
+Require Import Cava.Lib.MultiplexersProperties.
 Require Import Cava.Util.List.
 Require Import Cava.Util.Tactics.
-Import ListNotations Circuit.Notations.
+Import ListNotations Circuit.Notations MonadNotation.
 
-(* starting from scratch with retiming lemmas! Might not even need cequivn now. *)
+(* Start from scratch again. What do we really need? *)
 
-Fixpoint multi_loop {i o s}
-  : Circuit (i * ivalue s) (o * ivalue s) -> ivalue s -> Circuit i o :=
-  match s with
-  | ione t => fun c resetval => LoopInit resetval c
-  | ipair t1 t2 =>
-    fun (c : Circuit (i * (ivalue t1 * ivalue t2))
-                   (o * (ivalue t1 * ivalue t2)))
-      (resetvals : ivalue t1 * ivalue t2) =>
-      multi_loop
-        (multi_loop
-           (Comb (fun '(i,s1,s2) => ret (i,(s1,s2)))
-                 >==> c
-                 >==> Comb (fun '(o,(s1,s2)) => ret (o,s1,s2)))
-           (snd resetvals))
-        (fst resetvals)
-  end.
+(*
+All should be based on phase_retimed!
+- Move input delays over compose
+- Move state delays over feedback
+- Add delays to one end or the other, increment retiming number
+- retimed 0 0 <-> cequiv
+- Move delays over compose for loop-free circuits in general?
+- Move delays in/out of loops?
 
-Fixpoint loops_reset_state {i o} (c : Circuit i o)
-  : ivalue (signal:=combType) (loops_state c) :=
-  match c as c in Circuit i o return ivalue (loops_state c) with
-  | Comb _ => tt
-  | First f => loops_reset_state f
-  | Second f => loops_reset_state f
-  | Compose f g => (loops_reset_state f, loops_reset_state g)
-  | DelayInitCE r => tt
-  | LoopInitCE r body => (loops_reset_state body, r)
-  end.
+ *)
 
-(* counts # delays on the critical path *)
-Fixpoint cpath_delay {i o} (c : Circuit i o) : nat :=
+Lemma LoopInit_ignore_state {i o s} resetval (c : Circuit i o) :
+  cequiv (LoopInit (s:=s) resetval (First c)) c.
+Proof.
+  exists (fun s1 s2 => fst (snd s1) = s2). cbn [circuit_state LoopInit value].
+  split; [ reflexivity | ].
+  intros; destruct_products; cbn [fst snd] in *; subst.
+  cbn [step LoopInit]. simpl_ident.
+  repeat (destruct_pair_let; cbn [fst snd]).
+  split; reflexivity.
+Qed.
+
+Lemma LoopInit_merge {i1 o1 o2 s1 s2} r1 r2
+      (c1 : Circuit (i1 * s1) (o1 * s1))
+      (c2 : Circuit (o1 * s2) (o2 * s2)) :
+  cequiv (LoopInit r1 c1 >==> LoopInit r2 c2)
+         (LoopInit (s:=s1*s2)
+                   (r1, r2)
+                   ((Comb (i:=_*(_*_))
+                          (fun '(i,(s1,s2)) =>
+                             ret (i, s1, s2)))
+                      >==> First c1
+                      >==> (Comb (i:=_*_*_)
+                                 (fun '(o1,s1',s2) =>
+                                    ret (o1, s2, s1')))
+                      >==> First c2
+                      >==> (Comb (i:=_*_*_)
+                                 (fun '(o2,s2',s1') =>
+                                    ret (o2, (s1', s2')))))).
+Proof.
+  exists (fun s1 s2 =>
+       s2 = (tt, (tt, fst (snd (fst s1)), tt, fst (snd (snd s1)),
+                  tt, (snd (snd (fst s1)), snd (snd (snd s1)))))).
+  cbn [circuit_state reset_state LoopInit value].
+  split; [ reflexivity | ].
+  intros; destruct_products; cbn [fst snd] in *; subst.
+  simpl_ident. logical_simplify.
+  cbn [step LoopInit fst snd]. simpl_ident.
+  repeat (destruct_pair_let; cbn [fst snd]).
+  ssplit; reflexivity.
+Qed.
+
+Lemma First_LoopInit {i o s t} r
+      (c : Circuit (i * s) (o * s)) :
+  cequiv (First (t:=t) (LoopInit r c))
+         (LoopInit r
+                   ((Comb (i:=_*_*_)
+                          (fun '(i,t,s) => ret (i,s,t)))
+                      >==> First c
+                      >==> (Comb (i:=_*_*_)
+                                 (fun '(o,s,t) => ret (o,t,s))))).
+Proof.
+  exists (fun s1 s2 =>
+       s2 = (tt, (tt, fst (snd s1), tt, snd (snd s1)))).
+  cbn [circuit_state reset_state LoopInit value].
+  split; [ reflexivity | ].
+  intros; destruct_products; cbn [fst snd] in *; subst.
+  simpl_ident. logical_simplify.
+  cbn [step LoopInit fst snd]. simpl_ident.
+  repeat (destruct_pair_let; cbn [fst snd]).
+  ssplit; reflexivity.
+Qed.
+
+Lemma Second_LoopInit {i o s t} r
+      (c : Circuit (i * s) (o * s)) :
+  cequiv (Second (t:=t) (LoopInit r c))
+         (LoopInit r
+                   ((Comb (i:=_*_*_)
+                          (fun '(t,i,s) => ret (t,(i,s))))
+                      >==> Second c
+                      >==> (Comb (i:=_*(_*_))
+                                 (fun '(t,(o,s)) => ret (t,o,s))))).
+Proof.
+  exists (fun s1 s2 =>
+       s2 = (tt, (tt, fst (snd s1), tt, snd (snd s1)))).
+  cbn [circuit_state reset_state LoopInit value].
+  split; [ reflexivity | ].
+  intros; destruct_products; cbn [fst snd] in *; subst.
+  simpl_ident. logical_simplify.
+  cbn [step LoopInit fst snd]. simpl_ident.
+  repeat (destruct_pair_let; cbn [fst snd]).
+  ssplit; reflexivity.
+Qed.
+
+Lemma LoopInit_LoopInit {i o s1 s2} r1 r2
+      (c : Circuit (i * s1 * s2) (o * s1 * s2)) :
+  cequiv (LoopInit r1 (LoopInit r2 c))
+         (LoopInit (s:=s1*s2)
+                   (r1, r2)
+                   ((Comb (i:=_*(_*_))
+                          (fun '(i,(s1,s2)) =>
+                             ret (i, s1, s2)))
+                      >==> c
+                      >==> (Comb (i:=_*_*_)
+                                 (fun '(o,s1,s2) =>
+                                    ret (o, (s1, s2)))))).
+Proof.
+  exists (fun s1 s2 =>
+       s2 = (tt, (tt, fst (snd (fst (snd s1))), tt,
+                  (snd (snd s1), snd (snd (fst (snd s1))))))).
+  cbn [circuit_state reset_state LoopInit value].
+  split; [ reflexivity | ].
+  intros; destruct_products; cbn [fst snd] in *; subst.
+  simpl_ident. logical_simplify.
+  cbn [step LoopInit fst snd]. simpl_ident.
+  repeat (destruct_pair_let; cbn [fst snd]).
+  ssplit; reflexivity.
+Qed.
+
+Lemma LoopInitCE_LoopInit {i o s1 s2} r1 r2 (c : Circuit (i * s1 * s2) (o * s1 * s2)) :
+  cequiv (LoopInitCE r1 (LoopInit r2 c))
+         (LoopInit (s:=s2*s1)
+                   (r2, r1)
+                   ((Comb (i:=_*_*(_*_))
+                          (fun '(x, en, (s2, s1)) =>
+                             ret (en, s1, (x, s1, s2)))
+                          >==> Second c
+                          >==> (Comb (i:=Bit*s1*(o*s1*s2))
+                                     (o:=o*(s2*s1))
+                                     (fun '(en, s1, (y, s1', s2')) =>
+                                        s <- mux2 en (s1, s1') ;;
+                                        ret (y, (s2', s))))))).
+Proof.
+  exists (fun s1 s2 =>
+       s2 = (tt, (tt, fst (snd (fst s1)), tt,
+                  (snd (snd (fst s1)), snd s1)))).
+  cbn [circuit_state reset_state LoopInit value].
+  split; [ reflexivity | ].
+  intros; destruct_products; cbn [fst snd] in *; subst.
+  simpl_ident. logical_simplify.
+  cbn [step LoopInit fst snd]. simpl_ident.
+  repeat (destruct_pair_let; cbn [fst snd]).
+  simpl_ident. ssplit; reflexivity.
+Qed.
+
+Lemma extract_loops {i o} (c : Circuit i o) :
+  cequiv c (LoopInit (loops_reset_state c) (loopless c)).
+Proof.
+  induction c; cbn [loopless].
+  { rewrite LoopInit_ignore_state. reflexivity. }
+  { rewrite IHc1 at 1. rewrite IHc2 at 1.
+    apply LoopInit_merge. }
+  { rewrite IHc at 1. apply First_LoopInit. }
+  { rewrite IHc at 1. apply Second_LoopInit. }
+  { simpl_ident. rewrite IHc at 1.
+    apply LoopInitCE_LoopInit. }
+  { rewrite LoopInit_ignore_state. reflexivity. }
+Qed.
+
+Fixpoint is_loop_free {i o} (c : Circuit i o) : bool :=
   match c with
-  | Comb _ => 0
-  | First f => cpath_delay f
-  | Second f => cpath_delay f
-  | Compose f g => cpath_delay f + cpath_delay g
-  | DelayInitCE r => 1
-  | LoopInitCE r body => cpath_delay body
+  | Comb _ => true
+  | Compose f g => (is_loop_free f && is_loop_free g)%bool
+  | First f => is_loop_free f
+  | Second f => is_loop_free f
+  | DelayInitCE _ => true
+  | LoopInitCE _ _ => false
   end.
 
-Inductive is_loop_free : forall {i o}, Circuit i o -> Prop :=
-| is_loop_free_comb : forall {i o} (f : i -> cava o), is_loop_free (Comb f)
-| is_loop_free_first :
-    forall {i t o} f, is_loop_free f -> is_loop_free (@First _ _ i t o f)
-| is_loop_free_second :
-    forall {i t o} f, is_loop_free f -> is_loop_free (@Second _ _ i t o f)
-| is_loop_free_compose :
-    forall {i t o} f g, is_loop_free f -> is_loop_free g ->
-                   is_loop_free (@Compose _ _ i t o f g)
-| is_loop_free_delay : forall {t} r, is_loop_free (@DelayInitCE _ _ t r)
-.
-
-Definition extract_loops {i o} (c : Circuit i o) : Circuit i o :=
-  multi_loop (loopless c) (loops_reset_state c).
-
-Lemma is_loop_free_loopless {i o} (c : Circuit i o) : is_loop_free (loopless c).
-Proof. induction c; cbn [loopless]; repeat constructor; eauto. Qed.
-
-Lemma extract_loops_equiv {i o} (c : Circuit i o) : cequiv (extract_loops c) c.
-Proof.
+Lemma move_delays {i o} (iresets : value i) (oresets : value o) (c : Circuit i o) :
+  is_loop_free c = true ->
+  oresets = snd (step c (reset_state c) iresets) ->
+  cequiv (delays iresets >==> c) (c >==> delays oresets).
 Admitted.
 
-Lemma cequivn_reflexive_loop_free i o (c : Circuit i o) :
-  is_loop_free c -> cequivn (cpath_delay c) c c.
+Lemma delay_input {i o} n m (c1 c2 : Circuit i o) resets :
+  phase_retimed n m c1 (delays resets >==> c2) ->
+  phase_retimed n (S m) c1 c2.
+Admitted.
+
+Lemma ndelay_state {i o} n m (c1 c2 : Circuit i o) resets :
+  phase_retimed n m c1 (delays resets >==> c2) ->
+  phase_retimed n m c1 c2.
+Admitted.
+
+Lemma phase_retimed_cequiv_iff {i o} (c1 c2 : Circuit i o) :
+  phase_retimed 0 0 c1 c2 <-> cequiv c1 c2.
 Proof.
-  induction 1; cbn [cpath_delay].
-  { exists eq. cbn [circuit_state]. ssplit; intros.
-    all:destruct_lists_by_length; subst.
-    all:repeat lazymatch goal with x : unit |- _ => destruct x end.
-    all:ssplit; reflexivity. }
+  cbv [phase_retimed]. split; intros; logical_simplify.
+  { destruct_lists_by_length. cbn [ndelays] in *.
+    cbv [Par] in *. autorewrite with circuitsimpl in *.
+    rewrite <-(extract_loops c2) in *. assumption. }
+  { exists [], []. ssplit; [ reflexivity .. | ].
+    cbn [ndelays]. cbv [Par]. autorewrite with circuitsimpl.
+    rewrite <-extract_loops. assumption. }
+Qed.
+
+Axiom reassemble_state :
+  forall {i o} (c : Circuit i o), value (circuit_state (loopless c)) -> value (loops_state c) -> value (circuit_state c).
+
+Axiom loops_state_from_circuit_state :
+  forall {i o} (c : Circuit i o), value (circuit_state c) -> value (loops_state c).
+
+Global Instance Proper_phase_retimed {i o} :
+  Proper (eq ==> eq ==> cequiv ==> cequiv ==> iff) (@phase_retimed i o).
+Proof.
+  repeat intro. subst.
+  split; cbv [phase_retimed]; intros; logical_simplify.
   { lazymatch goal with
-    | H : cequivn _ _ _ |- _ => destruct H as [R [Hstart HR]]
+    | Heq : cequiv ?c1 ?c2, H : context [loopless ?c1] |- context [loopless ?c2] =>
+      destruct Heq as [R [Hstart Hpres]]
     end.
-    exists R; cbn [circuit_state]; ssplit; intros;
-      [ autorewrite with push_repeat_step; apply Hstart; length_hammer | ].
-    cbn [step]. repeat (destruct_pair_let; cbn [fst snd]).
-    destruct_products; cbn [fst snd].
-    specialize (HR _ _ ltac:(eassumption) ltac:(eassumption)).
-    logical_simplify. ssplit; congruence. }
-  { lazymatch goal with
-    | H : cequivn _ _ _ |- _ => destruct H as [R [Hstart HR]]
-    end.
-    exists R; cbn [circuit_state]; ssplit; intros;
-      [ autorewrite with push_repeat_step; apply Hstart; length_hammer | ].
-    cbn [step]. repeat (destruct_pair_let; cbn [fst snd]).
-    destruct_products; cbn [fst snd].
-    specialize (HR _ _ ltac:(eassumption) ltac:(eassumption)).
-    logical_simplify. ssplit; congruence. }
-  { lazymatch goal with
-    | H : cequivn _ _ f |- _ => destruct H as [R1 [Hstart1 HR1]]
-    end.
-    lazymatch goal with
-    | H : cequivn _ _ g |- _ => destruct H as [R2 [Hstart2 HR2]]
-    end.
-    exists (fun st1 st2 => R1 (fst st1) (fst st2) /\ R2 (snd st1) (snd st2)).
-    cbn [circuit_state]; ssplit; intros.
-    { ssplit.
-      { autorewrite with push_repeat_step. cbn [fst snd].
-        eapply state_relation_repeat_step_longer; eauto;
-        length_hammer. }
-      { erewrite <-(firstn_skipn (cpath_delay f) input).
-        rewrite !repeat_step_app.
-        autorewrite with push_repeat_step. cbn [fst snd].
-        erewrite state_relation_fold_left_accumulate_step
-          by (eauto; eapply Hstart1; length_hammer).
-        eapply Hstart2. length_hammer. } }
-    { cbn [step]. repeat (destruct_pair_let; cbn [fst snd]).
-      destruct_products; cbn [fst snd] in *.
-      specialize (HR1 _ _ ltac:(eassumption) ltac:(eassumption)).
-      lazymatch goal with
-      | |- context [step g _ ?i] =>
-        specialize (HR2 _ _ i ltac:(eassumption))
-      end.
-      logical_simplify. ssplit; congruence. } }
-  { exists eq. cbn [circuit_state].
-    ssplit; intros; [ | subst; ssplit; reflexivity ].
-    destruct_lists_by_length; subst.
-    autorewrite with push_repeat_step.
-    cbn [step]. repeat (destruct_pair_let; cbn [fst snd]).
-    (* damn it, doesn't work because delay might be disabled *)
-Abort.
-
-Lemma ndelays0_is_id {t} (c : Circuit t t) : is_ndelays 0 c -> c = Id.
-Proof. inversion 1; subst; reflexivity. Qed.
-
-Lemma phase_retimed_retimed_iff {i o} m (c1 c2 : Circuit i o) :
-  phase_retimed 0 m c1 c2 <-> retimed m c1 c2.
+    do 2 eexists; ssplit.
+    3:{
+      rewrite <-H1. rewrite H3.
+      exists (fun (s1 : unit * (value (circuit_state (ndelays _))
+                         * value (circuit_state (ndelays _))
+                         * value (circuit_state (loopless _))
+                         * value (loops_state _)))
+           (s2 : unit * (value (circuit_state (ndelays _))
+                         * value (circuit_state (ndelays _))
+                         * value (circuit_state (loopless _))
+                         * value (loops_state _))) =>
+           R (reassemble_state _ (snd (fst (snd s1))) (snd (snd s1)))
+             (reassemble_state _ (snd (fst (snd s2))) (snd (snd s2)))
+           /\ ndelays_get (fst (fst (fst (snd s1)))) = ndelays_get (fst (fst (fst (snd s2))))
+           /\ (Forall2
+                (fun v1 v2 =>
+                   exists u1 u2, R (reassemble_state _ u1 v1) (reassemble_state _ u2 v2))
+                (ndelays_get (snd (fst (fst (snd s1)))))
+                (ndelays_get (snd (fst (fst (snd s2))))))).
 Admitted.
-
-(*
-Lemma invert_delays'_par {t1 t2} (c : Circuit (ivalue (ipair t1 t2)) (ivalue (ipair t1 t2))) :
-  is_delays' _ c ->
-  exists d1 d2, is_delays' t1 d1 /\ is_delays' t2 d2 /\ c = Par d1 d2.
-Proof.
-  inversion 1. inversion_sigma; subst.
-  do 2 eexists; ssplit; eauto.
-  rewrite <-Eqdep_dec.eq_rect_eq_dec by apply itype_eq_dec.
-  reflexivity.
-Qed.
-
-Lemma invert_delays'_delay {t} (c : Circuit (ivalue (ione t)) (ivalue (ione t))) :
-  is_delays' _ c -> exists r, c = DelayInit r.
-Proof.
-  inversion 1. inversion_sigma; subst.
-  rewrite <-Eqdep_dec.eq_rect_eq_dec by apply itype_eq_dec.
-  eexists; reflexivity.
-Qed.
-
-Lemma split_delays {t1 t2} (c : Circuit (t1 * t2) (t1 * t2)) :
-  is_delays c ->
-  exists (d1 : Circuit t1 t1) (d2 : Circuit t2 t2),
-    is_delays d1 /\ is_delays d2 /\ c = Par d1 d2.
-Proof.
-  inversion 1. inversion_sigma; subst.
-  destruct t.
-  { eapply invert_delays'_delay in H2.
-    logical_simplify; subst.
-    Search unit.
-    inversion H. inversion_sigma.
-    cbn [ivalue] in *. subst.
-    rewrite H4 in *.
-    do 2 eexists.
-    rewrite f_equal_dep.
-  eapply split_delays' in H2.
-  rewrite H4 in *.
-  do 2 eexists.
-  rewrite <-Eqdep_dec.eq_rect_eq_dec by apply itype_eq_dec.
-Qed.
-
-
-Lemma split_ndelays {t1 t2} n (c : Circuit (t1 * t2) (t1 * t2)) :
-  is_ndelays n c ->
-  exists (d1 : Circuit t1 t1) (d2 : Circuit t2 t2),
-    is_ndelays n d1 /\ is_ndelays n d2 /\ cequiv c (Par d1 d2).
-Proof.
-  inversion 1.
-  induction 1.
-Qed.
-*)
-
-Lemma phase_retimed_LoopInit
-      {i o s} n m (c1 c2 : Circuit (i * combType s) (o * combType s)) r :
-  phase_retimed n m c1 c2 ->
-  phase_retimed (S n) m (LoopInit r (Second Delay >==> c1)) (LoopInit r c2).
-Proof.
-  intros [state_delays [input_delays [proj ?]]].
-  logical_simplify.
-  exists (Par Delay (Par state_delays Delay)).
-  exists (Comb (fun i => ret (i, defaultCombValue s))
-          >==> input_delays
-          >==> Comb (fun '(i,s) => ret i)).
-  cbn [loops_state LoopInit ivalue].
-Qed.
-
-(* phase_retimed n m c1 c2 -> is_ndelays m d ->
-   phase_retimed n m (Loop (Second d >==> c1)) (Loop c2) *)
-Print retimed.
-Print phase_retimed.
-(* retimed is NOT related to cequivn as stated, because cequivn says everything
-   will always stabilize after a certain number of inputs and that's just not
-   true within loops. equiv is actually weaker because it says they must be in
-   the same start state.
-
-   What about phase_retimed? That one *is* related, because we have the
-   guarantee that the circuit is loopless.
-
-   Actually, no it's not, because we could have *disabled* delays inside the
-   circuit and that would mean state could linger longer.
-
-
-   What we really need for loops is not quite cequivn; we need a guarantee that
-   after an equal input, N cycles later the circuits will produce an equal output.
-
- *)
-
-(* forall c, cequivn (ncycles c) c c *)
-(* forall c1 c2, cequiv c1 c2 -> ncycles c1 = ncycles c2 /\ cequivn (ncycles c1) c1 c2*)
-(* cequiv c1 c2 -> cequivn c1 c3 -> cequivn n c2 c3? *)
-
-
-(* is_delays c1 -> is_delays c2 -> cequivn 1 c1 c2 *)
-(* cequivn n c2 -> is_delays d1 -> is_delays d2 -> cequivn (S n) (c1 >==> d) (c2 >==> d) *)
-(* is_ndelays n c1 -> is_ndelays n c2 -> cequivn n c1 c2 *)
-
-(* retimed n c1 c2 -> is_delays d -> retimed (S n) (c1 >==> d) c2 *)
-(* retimed 0 c1 c2 <-> cequiv c1 c2 *)
-(* cequiv c1 c2 -> retimed n c1 c3 -> retimed n c2 c3 *)
-(* cequiv c1 c2 -> retimed n c3 c1 -> retimed n c3 c2 *)
-(* is_delays d -> exists d', is_delays d' /\ cequiv (d >==> c) (c >==> d') *)
-(* is_delays d1 -> is_delays d2  -> cequivn (c >==> d1) (c >==> d2) *)
-(* is_delays d -> is_delays d' -> cequivn 1 (d >==> c) (c >==> d') *)
-(* is_ndelays n d -> is_ndelays n d' -> cequivn n (d >==> c) (c >==> d') *)
-
-(* cequiv n c1 c2 -> retimed n c1 c3 -> retimed n c2 c3 *)
-
-(* is_delays d -> retimed n (c >==> d) *)
-(* is_delays d -> exists d', is_delays d' /\ cequiv (d >==> c) (c >==> d') *)
-
-(* retimed n c1 c2 <-> phase_retimed n 0 c1 c2 *)
-(* phase_retimed n m c1 c2 -> is_ndelays m d ->
-   phase_retimed n m (Loop (Second d >==> c1)) (Loop c2) *)
-
-
-
-
-
-
-
-
-
-
-
-
-
-
-
-
-
-
-
-
-
-
-
-
-
-
-
-
-
-
-
-
-
-
-Lemma retimed_cequiv_iff {i o} n (c1 c2 : Circuit i (ivalue o)) :
-  retimed n c1 c2 <-> (exists d, cequivn n d (ndelays n o)
-                          /\ cequiv c1 (c2 >==> d)).
-Proof.
-  (* do we need this lemma? *)
-Admitted.
-
-(*
-Lemma retimed0_cequiv_iff {i o} (c1 c2 : Circuit i (ivalue o)) :
-  retimed 0 c1 c2 -> cequiv c1 c2.
-Proof.
-  cbv [retimed ndelays]. autorewrite with circuitsimpl.
-  intros.
-  apply cequivn_cequiv.
-  split.
-  { intros [resetvals ?]. logical_simplify.
-    destruct resetvals; [ | cbn [length] in *; lia ].
-    cbn [ndelays fold_left] in *.
-    autorewrite with circuitsimpl in *. auto. }
-  { intros. exists nil. ssplit; [ reflexivity | ].
-    cbn [ndelays fold_left].
-    autorewrite with circuitsimpl. auto. }
-Qed.
-
-(* rephrasing of the definition of retimed that can be helpful when proving a
-   retimed goal *)
-Lemma retimed_cequiv {i o} n (c1 c2 : Circuit i (ivalue o)) resetvals :
-  cequiv c1 (c2 >==> ndelays o resetvals) ->
-  length resetvals = n ->
-  retimed n c1 c2.
-Proof. cbv [retimed]; intros; eauto. Qed.
- *)
-
-Lemma simulate_delays t input :
-  simulate (delays t) input = firstn (length input) (idefault t :: input).
-Proof.
-  revert input; induction t; intros; cbn [delays ivalue idefault];
-    autorewrite with push_simulate; [ reflexivity | ].
-  rewrite !IHt1, IHt2. autorewrite with push_length.
-  rewrite <-combine_firstn. cbn [combine].
-  rewrite combine_map_r, combine_map_l, combine_same.
-  rewrite !map_map. cbn [fst snd].
-  rewrite List.map_id_ext by (intros; symmetry; apply surjective_pairing).
-  reflexivity.
-Qed.
-Hint Rewrite @simulate_delays using solve [eauto] : push_simulate.
-
-Lemma delays_get_reset t  :
-  delays_get (reset_state (delays t)) = idefault t.
-Proof.
-  induction t; [ reflexivity | ].
-  cbn [delays delays_get Par reset_state fst snd].
-  rewrite IHt1, IHt2. reflexivity.
-Qed.
-
-Lemma delays_get_step t st input :
-  delays_get (fst (step (delays t) st input)) = input.
-Proof.
-  induction t; [ reflexivity | ].
-  cbn [delays delays_get Par step fst snd].
-  repeat (destruct_pair_let; cbn [fst snd]).
-  rewrite IHt1, IHt2, <-surjective_pairing.
-  reflexivity.
-Qed.
-
-Lemma step_delays t st input :
-  snd (step (delays t) st input) = delays_get st.
-Proof.
-  induction t; [ reflexivity | ].
-  cbn [delays delays_get Par step fst snd].
-  repeat (destruct_pair_let; cbn [fst snd]).
-  rewrite IHt1, IHt2. reflexivity.
-Qed.
-
-Lemma is_delays_cequivn t (c1 c2 : Circuit t t) :
-  is_delays c1 -> is_delays c2 -> cequivn 1 c1 c2.
-Admitted.
-
-Lemma is_ndelays_cequivn t n (c1 c2 : Circuit t t) :
-  is_ndelays n c1 -> is_ndelays n c2 -> cequivn n c1 c2.
-Admitted.
-
-Lemma fold_left_accumulate_step_DelayInit t (resetval : combType t) input st :
-  fold_left_accumulate (step (DelayInit resetval)) input st
-  = firstn (length input) (snd st :: input).
-Proof.
-  revert st. cbv [DelayInit]. simpl_ident. cbn [circuit_state step].
-  induction input; intros; [ reflexivity | ].
-  autorewrite with push_length push_firstn push_fold_acc.
-  destruct_products; cbn [fst snd]. erewrite IHinput.
-  reflexivity.
-Qed.
-
-Lemma move_DelayInit i o n (c1 c2 : Circuit (combType i) (combType o))
-      resetvali resetvalo :
-  cequivn n c1 c2 ->
-  cequivn (S n) (c1 >==> DelayInit resetvalo) (DelayInit resetvali >==> c2).
-Proof.
-  intros [R [? HR]].
-  exists (fun (st1 : circuit_state c1 * (unit * combType o))
-       (st2 : unit * combType i * circuit_state c2) =>
-       R (fst st1) (fst (step c2 (snd st2) (snd (fst st2))))
-       /\ snd (step c2 (snd st2) (snd (fst st2))) = snd (snd st1)).
-  ssplit.
-  { cbn [circuit_state]; intro input; intros.
-    destruct input using rev_ind; [ cbn [length] in *; lia | ].
-    clear IHinput.
-    autorewrite with push_repeat_step push_fold_acc; cbn [fst snd].
-    rewrite fold_left_accumulate_step_DelayInit.
-    autorewrite with push_length. rewrite ?Nat.add_1_r.
-    autorewrite with push_firstn natsimpl listsimpl.
-    cbn [step DelayInit]. simpl_ident.
-    autorewrite with push_repeat_step.
-    ssplit.
-    { lazymatch goal with
-      | |- R (fst (step c1 ?s1 ?x)) (fst (step c2 ?s2 ?x)) =>
-        assert (R s1 s2)
-      end.
-      { Search repeat_step.
-        apply state_relation_repeat_step.
-      eapply HR.
-      rewrite fold_left_accumulate_step_DelayInit.
-      autorewrite with push_length. rewrite Nat.add_1_r.
-      autorewrite with push_firstn natsimpl listsimpl.
-      Search fold_left_accumulate.
-      Search repeat_step.
-      eapply H.
-    cbv [DelayInit]. cbn [step circuit_state]. simpl_ident.
-    ssplit.
-    { Search repeat_step.
-      eapply state_relation_repeat_step.
-    rewrite <-surjective_pairing.
-Qed.
-
-
-Lemma move_delays i o (c1 : Circuit i o) c2 c3 :
-  is_delays c2 -> is_delays c3 ->
-  cequivn 1 (c1 >==> c2) (c3 >==> c1).
-Proof.
-  revert c3; induction 1.
-  { destruct 1.
-    { 
-Qed.
-
-Lemma is_delays_cequivn_compose t n (c1 c2 c3 : Circuit t t) :
-  is_delays n c1 -> is_delays n c2 ->
-  cequivn d (c3 >==> c1) (c3 >==> c2) = cequivn (m - n).
-Admitted.
-
-Search cequivn.
-Lemma is_ndelays_cequivn_compose t n (c1 c2 c3 : Circuit t t) :
-  is_ndelays n c1 -> is_ndelays n c2 ->
-  cequivn n (c3 >==> c1) (c3 >==> c2) = cequivn (m - n).
-Admitted.
-
-Lemma retimed_cequivn i o n (c1 c2 c3 : Circuit i o) :
-  retimed n c1 c2 -> retimed n c1 c3 -> cequivn n c2 c3.
-Proof.
-  cbv [retimed]; intros. logical_simplify.
-  rewrite H2 in H1.
-  etransitivity.
-  { symmetry.
-  Search cequivn.
-Qed.
-
-Lemma move_delays i o n (c1 c2 : Circuit (ivalue i) (ivalue o)) :
-  cequivn n c1 c2 ->
-  cequivn (S n) (delays i >==> c1) (c2 >==> delays o).
-Proof.
-  intros.
-  etransitivity.
-  (* transitivity, replace delays with some delays that have the reset values for c1 (defaults) *)
-  (* OR transitivity, then use cequivn compose-delay lemmas *)
-  eapply cequivn_compose with (n0:=1) (m:=n).
-  
-  intros [R [? ?]].
-  exists (fun (st1 : circuit_state (delays i) * circuit_state c1)
-       (st2 : circuit_state c2 * circuit_state (delays o)) =>
-       exists st1',
-         step c1 (snd st1) (delays_get (fst st1)) = (st1', delays_get (snd st2))).
-  ssplit.
-  { cbn [circuit_state]. intro input; intros.
-    destruct input using rev_ind; [ cbn [length] in *; lia | ].
-    clear IHinput. autorewrite with push_repeat_step.
-    rewrite !fold_left_accumulate_snoc. cbn [fst snd].
-    autorewrite with push_repeat_step push_fold_acc.
-    destruct_products; cbn [fst snd] in *.
-    rewrite !step_delays, !delays_get_step.
-    rewrite H0.
-    eexists.
-    
-    repeat (destruct_pair_let; cbn [fst snd]).
-    rewrite !delays_get_step, !step_delays.
-  { cbn. rewrite !delays_get_reset.
-    destruct (step c (reset_state c) resetvalsi); cbn [fst snd] in *.
-    logical_simplify; subst. reflexivity. }
-  { cbn [circuit_state step]; intros *. intro Hstep.
-    destruct_products; cbn [fst snd] in *.
-    repeat (destruct_pair_let; cbn [fst snd]).
-    logical_simplify. rewrite !delays_get_step, !step_delays.
-    rewrite Hstep. cbn [fst snd]. rewrite <-surjective_pairing.
-    ssplit; reflexivity. }
-Qed.
-
-Lemma move_delays i o (c : Circuit (ivalue i) (ivalue o)) resetvalsi resetvalso :
-  (* step c applied to resetvals from resetstate needs to result in reset
-     state; otherwise first results don't match *)
-  step c (reset_state c) resetvalsi = (reset_state c, resetvalso) ->
-  cequiv (delays i resetvalsi >==> c)
-         (c >==> delays o resetvalso).
-Proof.
-  intro Hreset.
-  exists (fun (st1 : circuit_state (delays i resetvalsi) * circuit_state c)
-       (st2 : circuit_state c * circuit_state (delays o resetvalso)) =>
-       step c (snd st1) (delays_get (fst st1)) = (fst st2, delays_get (snd st2))).
-  ssplit.
-  { cbn. rewrite !delays_get_reset.
-    destruct (step c (reset_state c) resetvalsi); cbn [fst snd] in *.
-    logical_simplify; subst. reflexivity. }
-  { cbn [circuit_state step]; intros *. intro Hstep.
-    destruct_products; cbn [fst snd] in *.
-    repeat (destruct_pair_let; cbn [fst snd]).
-    logical_simplify. rewrite !delays_get_step, !step_delays.
-    rewrite Hstep. cbn [fst snd]. rewrite <-surjective_pairing.
-    ssplit; reflexivity. }
-Qed.
-
-Lemma ndelays_cons t resetvals r0 :
-  cequiv (ndelays t (r0 :: resetvals)) (ndelays t resetvals >==> delays t r0).
-Proof. reflexivity. Qed.
-
-Lemma ndelays_snoc t resetvals r0 :
-  cequiv (ndelays t (resetvals ++ [r0])) (delays t r0 >==> ndelays t resetvals).
-Proof.
-  revert r0. induction resetvals; intros.
-  { cbn [app ndelays]. autorewrite with circuitsimpl. reflexivity. }
-  { cbn [app ndelays]. rewrite IHresetvals, Compose_assoc.
-    reflexivity. }
-Qed.
-
-Lemma simulate_ndelays t resetvals input :
-  simulate (ndelays t resetvals) input
-  = firstn (length input) (resetvals ++ input).
-Proof.
-  revert input; induction resetvals; intros.
-  { autorewrite with push_simulate listsimpl push_firstn.
-    reflexivity. }
-  { rewrite ndelays_cons.
-    autorewrite with push_simulate push_length.
-    rewrite IHresetvals, <-app_comm_cons.
-    destruct input; [ reflexivity | ].
-    autorewrite with push_length push_firstn natsimpl.
-    apply Min.min_case_strong; intros; [ | reflexivity ].
-    autorewrite with natsimpl push_firstn listsimpl.
-    reflexivity. }
-Qed.
-Hint Rewrite @simulate_ndelays using solve [eauto] : push_simulate.
-
-Global Instance Proper_retimed i o :
-  Proper (eq ==> cequiv ==> cequiv ==> iff) (@retimed i o).
-Proof.
-  repeat intro. cbv [retimed].
-  split; intros; logical_simplify; subst;
-    eexists; (ssplit; [ reflexivity | ]).
-  all:repeat match goal with H : cequiv _ _ |- _ => rewrite H in * end.
-  all:reflexivity.
-Qed.
-
-Global Instance Reflexive_retimed0 i o : Reflexive (@retimed i o 0) | 10.
-Proof.
-  repeat intro; subst.
-  exists []; ssplit; [ reflexivity | ].
-  cbn [ndelays]. autorewrite with circuitsimpl.
-  reflexivity.
-Qed.
-
-Lemma retimed_step_r {i o} n (c1 c2 : Circuit i (ivalue o)) resetvals :
-  retimed n c1 (c2 >==> delays o resetvals) ->
-  retimed (S n) c1 c2.
-Proof.
-  intros. cbv [retimed] in *. logical_simplify; subst.
-  eexists (_++ [_]). autorewrite with push_length.
-  rewrite Nat.add_1_r. ssplit; [ reflexivity | ].
-  rewrite ndelays_snoc, Compose_assoc. eauto.
-Qed.
-
-Lemma retimed_transitivity {i o} n m (c1 c2 c3 : Circuit i (ivalue o)) :
-  retimed n c1 c2 ->
-  retimed m c2 c3 ->
-  retimed (n+m) c1 c3.
-Proof.
-  revert c1 c2 c3 n; induction m; intros *.
-  { rewrite retimed0_cequiv_iff.
-    autorewrite with natsimpl.
-    intros ? Heq. rewrite <-Heq; eauto. }
-  { intros ? [vals [? Heq]]. rewrite Nat.add_succ_r.
-    destruct vals using rev_ind; [ cbn [length] in *; lia | ].
-    eapply retimed_step_r. eapply IHm; eauto; [ ].
-    rewrite ndelays_snoc, !Compose_assoc in *.
-Abort.
-
-
-(*
-
-Can we prove that for every circuit, there exists n, c2 such that retimed n c1 (Comb c2)?
-
-If so, maybe we can prove move_ndelays for Comb only, and use that to prove retimed_step_l...
- *)
-
-Print retimed.
-(* need to be equivalent to c2 >==> delays
-
-   (delays >==> c2) will be equivalent to starting c2 at the state that results
-   from the reset value of the delays
-
-   (c2 >==> delays) will be just starting c2 as usual and then adding some
-   different outputs to the beginning, which is why it's different
-
-   R : circuit_state c1 -> ivalue i -> circuit_state c2 -> Prop
-
-   R (reset_state c1) resetvalsi (reset_state c2)
-
-   preserved_over_step c1 (delays >==> c2) R
-
-   need to prove exists R' : circuit_state c1 -> ivalue o -> circuit_state c2 ->
-   Prop such that R' (reset_state c1) resetvalso (reset_state c2) and
-   preserved_over_step c1 (c2 >==> delays) R'
-
-
-   IDEA: Can this be proven the *other* way around? i.e. if retimed means the
-   delay is tacked on the front, then can we prove the delay can be tacked on
-   the end?
-
-   we can get the values from running the circuit; right now we have to prove
-   the inputs exist
-
-   potential problem still: the state of the circuit for input 0 for delays >==>
-   c2 would still be the state after getting all the reset values, while the
-   state for c2 >==> delays would be the reset state first
- *)
-Lemma retimed_step_l {i o} n (c1 c2 : Circuit (ivalue i) (ivalue o)) resetvals :
-  retimed n c1 (delays i resetvals >==> c2) ->
-  retimed (S n) c1 c2.
-Proof.
-  intro Hretimed. pose proof Hretimed.
-  destruct Hretimed as [? [? [R ?]]].
-  logical_simplify; subst.
-  eapply retimed_step_r.
-  cbn [ndelays]. rewrite Compose_assoc.
-  ssplit.
-  2:{
-    cbn [circuit_state reset_state] in *.
-    exists (fun (st1 : circuit_state c1)
-         (st2 : circuit_state c2 * circuit_state (ndelays _ _)
-                * circuit_state (delays _ _)) =>
-         exists (vali : circuit_state (delays i resetvals)),
-           R st1 (vali, fst (fst st2), snd (fst st2))).
-    ssplit; [ eauto | ]. cbn [circuit_state].
-    intros; logical_simplify.
-    destruct_products; cbn [fst snd] in *.
-    ssplit.
-    { cbn.
-      repeat destruct_pair_let; cbn [fst snd].
-
-
-    
-  rewrite move_delays in H0.
-  ssplit; [ reflexivity | ].
-  rewrite ndelays_snoc, Compose_assoc. eauto.
-Qed.
-
-Lemma move_delays_retimed {i o} n (c1 c2 : Circuit (ivalue i) (ivalue o))
-      resetvalsi resetvalso :
-  retimed (S n) c1 (delays i resetvalsi >==> c2) ->
-  retimed (S n) c1 (c2 >==> delays o resetvalso).
-Proof.
-  intros [vals [? Hequiv]]. (* destruct Hequiv as [R [? ?]]]]. *)
-  destruct vals as [|v0 vals]; [ cbn [length] in *; lia | ].
-  cbn [ndelays circuit_state reset_state] in *.
-  
-Qed.
-
 
 Require Import Coq.derive.Derive.
 
+Local Ltac simpl_resets :=
+  cbn [step fst snd defaultValue default_value
+            CombinationalSemantics defaultSignal defaultCombValue].
+
 Derive pipelined_nand
-       SuchThat (retimed (o:=ione Bit) 2 pipelined_nand
-                         (Comb and2 >==> Comb inv))
+       SuchThat (phase_retimed
+                   0 2 pipelined_nand
+                   (Comb (i:=Bit*Bit) (o:=Bit) and2
+                         >==> Comb (o:=Bit) inv))
        As pipelined_nand_correct.
 Proof.
-  eapply retimed_step; [ reflexivity | ].
-  eapply retimed_step; [ reflexivity | ].
-  apply retimed0_cequiv_iff.
-  rewrite <-move_delays with (i:=ipair (ione Bit) (ione Bit))
-    by (cbn; repeat destruct_pair_let; reflexivity).
-  rewrite <-Compose_assoc.
-  rewrite <-move_delays with (i:=ione Bit)
-    by (cbn; repeat destruct_pair_let; reflexivity).
-  instantiate (1:=((false,false) : ivalue (signal:=combType) (ipair (ione Bit) (ione Bit)))).
-  cbn [fst snd andb delays]. autorewrite with circuitsimpl.
-  rewrite !Compose_assoc. subst pipelined_nand.
-  reflexivity.
+  (* insert a delay *)
+  eapply delay_input with (resets:=defaultValue).
+  (* move the delay to the end of the circuit *)
+  erewrite move_delays with (oresets:=true : value Bit) by reflexivity.
+  (* insert another delay *)
+  eapply delay_input with (resets:=defaultValue).
+  (* move the delay in between the and2 and inv *)
+  rewrite !Compose_assoc.
+  erewrite move_delays with (oresets:=false : value Bit) by reflexivity.
+  (* reflexivity *)
+  apply phase_retimed_cequiv_iff.
+  subst pipelined_nand; reflexivity.
 Qed.
 Print pipelined_nand.
+Check pipelined_nand_correct.
 
-Lemma ndelays_get_reset t resetvals :
-  ndelays_get (reset_state (ndelays t resetvals)) = resetvals.
+Definition cipher_middle_round
+           {state key : type}
+           (sbytes : Circuit state state)
+           (shrows : Circuit state state)
+           (mxcols : Circuit state state)
+           (add_rk : Circuit (state * key) state)
+  : Circuit (state * key) state :=
+  First (sbytes >==> shrows >==> mxcols) >==> add_rk.
+
+Derive retimed_cipher_middle_round
+       SuchThat
+       (forall {state key} n
+          (sbytes retimed_sbytes shrows mxcols : Circuit state state)
+          (add_rk : Circuit (state * key) state),
+           phase_retimed 0 n retimed_sbytes sbytes ->
+           phase_retimed
+             n 0
+             (retimed_cipher_middle_round
+                state key retimed_sbytes shrows mxcols add_rk)
+             (cipher_middle_round sbytes shrows mxcols add_rk))
+       As retimed_cipher_middle_round_correct.
 Proof.
-  induction resetvals; [ reflexivity | ].
-  cbn [ndelays ndelays_get delays_get reset_state fst snd].
-  rewrite delays_get_reset, IHresetvals.
-  reflexivity.
+  intros. cbv [cipher_middle_round].
+  autorewrite with circuitsimpl.
+  cbv [phase_retimed] in * |- . logical_simplify.
+  destruct_lists_by_length. cbn [ndelays] in *.
+  cbv [Par] in *; autorewrite with circuitsimpl in *.
+  
+
+
+  
+  (* insert a delay *)
+  eapply delay_input with (resets:=defaultValue).
+  (* move the delay to the end of the circuit *)
+  erewrite move_delays with (oresets:=true : value Bit) by reflexivity.
+  (* insert another delay *)
+  eapply delay_input with (resets:=defaultValue).
+  (* move the delay in between the and2 and inv *)
+  rewrite !Compose_assoc.
+  erewrite move_delays with (oresets:=false : value Bit) by reflexivity.
+  (* reflexivity *)
+  apply phase_retimed_cequiv_iff.
+  subst pipelined_nand; reflexivity.
 Qed.
-
-Lemma step_ndelays t resetvals st input :
-  snd (step (ndelays t resetvals) st input) = hd input (ndelays_get st).
-Proof.
-  induction resetvals; [ reflexivity | ].
-  cbn [ndelays ndelays_get step].
-  repeat (destruct_pair_let; cbn [fst snd]).
-  rewrite IHresetvals, step_delays. reflexivity.
-Qed.
-
-Lemma hd_snoc {A} d (l : list A) : hd d (l ++ [d]) = hd d l.
-Proof. destruct l; reflexivity. Qed.
-
-Lemma ndelays_get_step t resetvals st input :
-  ndelays_get (fst (step (ndelays t resetvals) st input))
-  = tl (ndelays_get st ++ [input]).
-Proof.
-  induction resetvals; [ reflexivity | ].
-  cbn [ndelays ndelays_get step fst snd].
-  repeat (destruct_pair_let; cbn [fst snd]).
-  rewrite delays_get_step, IHresetvals, step_ndelays.
-  rewrite <-app_comm_cons. cbn [hd tl].
-  etransitivity; [ | symmetry; apply eta_list; length_hammer ].
-  rewrite hd_snoc. reflexivity.
-Qed.
-
-Lemma move_ndelays i o (c : Circuit (ivalue i) (ivalue o)) resetvalsi resetvalso :
-  (*
-  (* step c applied to resetvals from resetstate needs to result in reset
-     state; otherwise first results don't match *)
-  step c (reset_state c) resetvalsi = (reset_state c, resetvalso) ->*)
-  cequiv (ndelays i resetvalsi >==> c)
-         (c >==> ndelays o resetvalso).
-Proof.
-  assert (length resetvalsi = length resetvalso) by admit.
-  revert c; revert dependent resetvalso;
-    induction resetvalsi; destruct resetvalso; intros;
-    cbn [length] in *; try lia; [ | ].
-  { cbn [ndelays]. autorewrite with circuitsimpl. reflexivity. }
-  { cbn [ndelays]. rewrite Compose_assoc.
-    erewrite <-(move_delays _ o).
-    2:{
-      cbn. repeat destruct_pair_let.
-      rewrite !step_ndelays.
-      rewrite ndel
-      f_equal. 1:f_equal.
-      
-      rewrite <-surjective_pairing.
-    rewrite <-(Compose_assoc _ _ _ _ (ndelays _ _)).
-    rewrite IHresetvalsi.
-    
-    Check move_delays.
-  intro Hreset.
-  exists (fun (st1 : circuit_state (delays i resetvalsi) * circuit_state c)
-       (st2 : circuit_state c * circuit_state (delays o resetvalso)) =>
-       step c (snd st1) (delays_get (fst st1)) = (fst st2, delays_get (snd st2))).
-  ssplit.
-  { cbn. rewrite !delays_get_reset.
-    destruct (step c (reset_state c) resetvalsi); cbn [fst snd] in *.
-    logical_simplify; subst. reflexivity. }
-  { cbn [circuit_state step]; intros *. intro Hstep.
-    destruct_products; cbn [fst snd] in *.
-    repeat (destruct_pair_let; cbn [fst snd]).
-    logical_simplify. rewrite !delays_get_step, !step_delays.
-    rewrite Hstep. cbn [fst snd]. rewrite <-surjective_pairing.
-    ssplit; reflexivity. }
-Qed.
-
-Lemma simulate_retimed
-      {i o} (n : nat) (c1 c2 : Circuit i (ivalue (signal:=combType) o)) input :
-  retimed n c1 c2 ->
-  skipn n (simulate c1 input) = firstn (length input - n) (simulate c2 input).
-Proof.
-  intros [? [? Heq]]. rewrite Heq.
-  autorewrite with push_simulate push_length.
-  rewrite skipn_firstn_comm. subst.
-  autorewrite with push_skipn natsimpl.
-  reflexivity.
-Qed.
-
-Lemma retimed_compose A B C n m
-      (c1 c2 : Circuit A (ivalue B)) (c3 c4 : Circuit (ivalue B) (ivalue C)) :
-  retimed n c1 c2 -> retimed m c3 c4 -> retimed (n+m) (c1 >==> c3) (c2 >==> c4).
-Proof.
-  intros [? [? Heq12]] [? [? Heq34]]. rewrite Heq12, Heq34.
-Qed.
-
-
-
-
-
-
-
-
-
-
-
-
-
-
-
-
-
-
-
-
-(*
-Lemma retimed_sum {i o} (n m: nat) (c1 c2 c3 : Circuit i o) :
-  retimed (n+m) c1 c2 -> retimed n c1 c3 -> retimed m c2 c3.
-Proof.
-  intros [R12 [? H12]]. intros [R13 [? H13]].
-  exists (fun i (st2 : circuit_state c2) (st3 : circuit_state c3) =>
-       exists st1, R12 i st1 st2
-              /\ R13 (Nat.modulo (i*m) n) st1 st3).
-  ssplit.
-  { exists (reset_state c1). ssplit; eauto.
-Qed.
-*)
-
-(*
-Lemma retimed_delays1_l_iff {i o} (n : nat) (c1 c2 : Circuit (ivalue i) o) :
-  retimed 1 c1 c2
-  <-> (exists resetvals : ivalue i,
-        cequiv c1 (delays i resetvals >==> c2)).
-Admitted.
- *)
-
-(*
-the second part matches every m cycles
-the first part matches every n cycles
-
-assume m=2, n=3
-
-0:reset
-2:second part matches
-3:first part matches
-4:second part matches
-6:first part matches
-??????
-ahhhh, the second part matches only m cycles *after its input matches*
-
-
-
-if we are i steps away from matching...
-
-if i <= m,
- the second part is i steps away from matching
-else
- second part unclear but does have an R
-
-
- *)
-
-Lemma retimed_compose A B C n m (c1 c2 : Circuit A B) (c3 c4 : Circuit B C) :
-  retimed n c1 c2 -> retimed m c3 c4 -> retimed (n+m) (c1 >==> c3) (c2 >==> c4).
-Proof.
-  intros [R12 [? H12]] [R34 [? H34]].
-  exists (fun i st1 st2 =>
-       R12 (i - m) (fst st1) (fst st2)
-       /\ R34 i (snd st1) (snd st2)).
-  cbn [reset_state fst snd].
-  ssplit;
-    [ autorewrite with natsimpl;
-      solve [eauto] | | ].
-  { 
-  cbn [circuit_state]. intros.
-  destruct_products; cbn [fst snd] in *.
-  logical_simplify. destruct_one_match.
-  { autorewrite with natsimpl in *.
-    cbn [step]. repeat (destruct_pair_let; cbn [fst snd]).
-    specialize (H34 0 _ _ (ltac:(eassumption)) (ltac:(lia))
-                    (ltac:(eassumption))).
-    cbn iota in H34. destruct H34 as [H34 ?].
-    rewrite H34 in *.
-  { 
-Qed.
-
-Lemma retimed_succ {i o} n (c1 c2 : Circuit (ivalue i) o) :
-  retimed (S n) c1 c2 ->
-  exists resetvals, retimed n c1 (delays i resetvals >==> c2).
-Proof.
-Qed.
-
-Lemma retimed_ndelays_l_iff {i o} (n : nat) (c1 c2 : Circuit (ivalue i) o) :
-  retimed n c1 c2 <-> (exists resetvals : list (ivalue i),
-                        length resetvals = n
-                        /\ cequiv c1 (ndelays i resetvals >==> c2)).
-Proof.
-  split.
-  { revert i o c1 c2; induction n; intros *.
-    { rewrite retimed_cequiv_iff.
-      intros. exists nil. cbn [ndelays fold_left].
-      autorewrite with circuitsimpl.
-      ssplit; eauto. }
-    {
-      (* retimed (S n) c1 c2 -> exists c3, retimed n c1 c3 /\ cequiv c3 (delays >==> c2) *)
-      
-      intros [R [? HR]]. logical_simplify.
-    
-
-    (*
-      equivalence state relation should say that R 0 holds on the last?
-    *)
-
-    evar (r: list (ivalue (signal:=combType) i)).
-    exists r. ssplit.
-    2:{
-      exists (fun (st1 : circuit_state c1)
-           (st2 : circuit_state (ndelays i r) * circuit_state c2) =>
-           R 0 st1 (snd st2)).
-      
-Qed.
-
+Print pipelined_nand.
+Check pipelined_nand_correct.
